Update to Cancun test and start cv approach to proof

vfmTestScript.sml
@@ -2,12 +2,11 @@ open HolKernel boolLib bossLib Parse wordsLib
      whileTheory
      vfmTypesTheory vfmExecutionTheory
      vfmStateTheory vfmContextTheory
-     vfmOperationTheory
-     cv_transLib cv_stdTheory cv_computeLib;
-open cv_primTheory byteTheory;
+     vfmOperationTheory vfmComputeTheory
+     cv_transLib cv_stdTheory cv_computeLib
+     cv_primTheory byteTheory;
 
 val _ = new_theory "vfmTest";
-
 
 (* TODO: move/replace *)
 Definition hex_to_bytes_def:
@@ -22,10 +21,48 @@ val _ = cv_auto_trans hex_to_bytes_def;
 
 (* cv_eval “hex_to_bytes "693c61390000000000000000000000000000000000000000000000000000000000000000"” *)
 
-(* BlockchainTests/GeneralStateTests/VMTests/vmArithmeticTest/add.json *)
+Definition empty_accounts_def:
+  empty_accounts (a: address) = empty_account_state
+End
 
-Definition add_d0g0v0_Shanghai_transaction_def:
-  add_d0g0v0_Shanghai_transaction =
+Theorem build_spt_empty_accounts[simp]:
+  ∀n. build_spt empty_account_state n empty_accounts = LN
+Proof
+  Induct \\ rw[build_spt_def]
+  \\ gs[empty_accounts_def]
+QED
+
+Theorem empty_accounts_cv_rep[cv_rep]:
+  from_evm_accounts empty_accounts = Num 0
+Proof
+  rw[from_evm_accounts_def, from_sptree_sptree_spt_def]
+QED
+
+(* TODO:
+initial_access_sets_def
+
+val () = cv_auto_trans initial_state_def;
+*)
+
+(*
+https://github.com/ethereum/tests
+commit 08839f5 (taken from the develop branch)
+BlockchainTests/GeneralStateTests/VMTests/vmArithmeticTest/add.json
+*)
+
+Definition add_d0g0v0_Cancun_block_def:
+  add_d0g0v0_Cancun_block =
+  <| number := 0x01
+   ; baseFee := 0x0a
+   ; timeStamp := 0x03e8
+   ; coinBase := n2w 0x2adc25665018aa1fe0e6bc666dac8fc2697ff9ba
+   ; gasLimit := 0x05f5e100
+   ; prevRandao := n2w 0x00 (* not sure - using the difficulty *)
+  |>
+End
+
+Definition add_d0g0v0_Cancun_transaction_def:
+  add_d0g0v0_Cancun_transaction =
   <| from := n2w 0xa94f5374fce5edbc8e2a8697c15331677e6ebf0b
    ; to   := n2w 0xcccccccccccccccccccccccccccccccccccccccc
    ; data := hex_to_bytes $ CONCAT [
@@ -39,9 +76,16 @@ Definition add_d0g0v0_Shanghai_transaction_def:
    |>
 End
 
-Definition add_d0g0v0_Shanghai_pre_def:
-  add_d0g0v0_Shanghai_pre a =
-  if a = n2w 0x0000000000000000000000000000000000001000 then
+Definition add_d0g0v0_Cancun_pre_def:
+  add_d0g0v0_Cancun_pre =
+  update_account (
+  update_account (
+  update_account (
+  update_account (
+  update_account (
+  update_account (
+  update_account empty_accounts
+    (n2w 0x0000000000000000000000000000000000001000)
     <| nonce := 0x00
      ; balance := 0x0ba1a9ce0ba1a9ce
      ; storage := empty_storage
@@ -51,7 +95,8 @@ Definition add_d0g0v0_Shanghai_pre_def:
                  ;"fffffffffffffffffffffffffffffffffffffff"
                  ;"fffffffffffffff0160005500"]
      |>
-  else if a = n2w 0x0000000000000000000000000000000000001001 then
+  )
+    (n2w 0x0000000000000000000000000000000000001001)
     <| nonce := 0x00
      ; balance := 0x0ba1a9ce0ba1a9ce
      ; storage := empty_storage
@@ -59,7 +104,8 @@ Definition add_d0g0v0_Shanghai_pre_def:
                  ["60047fffffffffffffffffffffffffffffffffff"
                  ;"ffffffffffffffffffffffffffffff0160005500"]
      |>
-  else if a = n2w 0x0000000000000000000000000000000000001002 then
+  )
+    (n2w 0x0000000000000000000000000000000000001002)
     <| nonce := 0x00
      ; balance := 0x0ba1a9ce0ba1a9ce
      ; storage := empty_storage
@@ -67,13 +113,15 @@ Definition add_d0g0v0_Shanghai_pre_def:
                  ["60017fffffffffffffffffffffffffffffffffff"
                  ;"ffffffffffffffffffffffffffffff0160005500"]
      |>
-  else if a = n2w 0x0000000000000000000000000000000000001003 then
+  )
+    (n2w 0x0000000000000000000000000000000000001003)
     <| nonce := 0x00
      ; balance := 0x0ba1a9ce0ba1a9ce
      ; storage := empty_storage
      ; code := hex_to_bytes "600060000160005500"
      |>
-  else if a = n2w 0x0000000000000000000000000000000000001004 then
+  )
+    (n2w 0x0000000000000000000000000000000000001004)
     <| nonce := 0x00
      ; balance := 0x0ba1a9ce0ba1a9ce
      ; storage := empty_storage
@@ -81,24 +129,32 @@ Definition add_d0g0v0_Shanghai_pre_def:
                   ["7fffffffffffffffffffffffffffffffffffffff"
                   ;"ffffffffffffffffffffffffff60010160005500"]
      |>
-  else if a = n2w 0xa94f5374fce5edbc8e2a8697c15331677e6ebf0b then
+  )
+    (n2w 0xa94f5374fce5edbc8e2a8697c15331677e6ebf0b)
     <| nonce := 0x00
      ; balance := 0x0ba1a9ce0ba1a9ce
      ; storage := empty_storage
      ; code := []
      |>
-  else if a = n2w 0xcccccccccccccccccccccccccccccccccccccccc then
+  )
+    (n2w 0xcccccccccccccccccccccccccccccccccccccccc)
     <| nonce := 0x00
      ; balance := 0x0ba1a9ce0ba1a9ce
      ; storage := empty_storage
      ; code := hex_to_bytes "600060006000600060006004356110000162fffffff100"
      |>
-  else empty_account_state
 End
 
-Definition add_d0g0v0_Shanghai_post_def:
-  add_d0g0v0_Shanghai_post a =
-  if a = n2w 0x0000000000000000000000000000000000001000 then
+Definition add_d0g0v0_Cancun_post_def:
+  add_d0g0v0_Cancun_post =
+  update_account (
+  update_account (
+  update_account (
+  update_account (
+  update_account (
+  update_account (
+  update_account empty_accounts
+    (n2w 0x0000000000000000000000000000000000001000)
     <| nonce := 0x00
      ; balance := 0x0ba1a9ce0ba1a9ce
      ; storage := (n2w 0x00 =+ n2w 0xfffffffffffffffffffffffffffffffffffffffffffffffffffffffffffffffe) empty_storage
@@ -108,7 +164,8 @@ Definition add_d0g0v0_Shanghai_post_def:
                  ;"fffffffffffffffffffffffffffffffffffffff"
                  ;"fffffffffffffff0160005500"]
      |>
-  else if a = n2w 0x0000000000000000000000000000000000001001 then
+  )
+    (n2w 0x0000000000000000000000000000000000001001)
     <| nonce := 0x00
      ; balance := 0x0ba1a9ce0ba1a9ce
      ; storage := empty_storage
@@ -116,7 +173,8 @@ Definition add_d0g0v0_Shanghai_post_def:
                  ["60047fffffffffffffffffffffffffffffffffff"
                  ;"ffffffffffffffffffffffffffffff0160005500"]
      |>
-  else if a = n2w 0x0000000000000000000000000000000000001002 then
+  )
+    (n2w 0x0000000000000000000000000000000000001002)
     <| nonce := 0x00
      ; balance := 0x0ba1a9ce0ba1a9ce
      ; storage := empty_storage
@@ -124,13 +182,15 @@ Definition add_d0g0v0_Shanghai_post_def:
                  ["60017fffffffffffffffffffffffffffffffffff"
                  ;"ffffffffffffffffffffffffffffff0160005500"]
      |>
-  else if a = n2w 0x0000000000000000000000000000000000001003 then
+  )
+    (n2w 0x0000000000000000000000000000000000001003)
     <| nonce := 0x00
      ; balance := 0x0ba1a9ce0ba1a9ce
      ; storage := empty_storage
      ; code := hex_to_bytes "600060000160005500"
      |>
-  else if a = n2w 0x0000000000000000000000000000000000001004 then
+  )
+    (n2w 0x0000000000000000000000000000000000001004)
     <| nonce := 0x00
      ; balance := 0x0ba1a9ce0ba1a9ce
      ; storage := empty_storage
@@ -138,35 +198,35 @@ Definition add_d0g0v0_Shanghai_post_def:
                   ["7fffffffffffffffffffffffffffffffffffffff"
                   ;"ffffffffffffffffffffffffff60010160005500"]
      |>
-  else if a = n2w 0xa94f5374fce5edbc8e2a8697c15331677e6ebf0b then
+  )
+    (n2w 0xa94f5374fce5edbc8e2a8697c15331677e6ebf0b)
     <| nonce := 0x01
      ; balance := 0x0ba1a9ce0b9aa781
      ; storage := empty_storage
      ; code := []
      |>
-  else if a = n2w 0xcccccccccccccccccccccccccccccccccccccccc then
+  )
+    (n2w 0xcccccccccccccccccccccccccccccccccccccccc)
     <| nonce := 0x00
      ; balance := 0x0ba1a9ce0ba1a9cf
      ; storage := empty_storage
      ; code := hex_to_bytes "600060006000600060006004356110000162fffffff100"
      |>
-  else empty_account_state
 End
 
-
-Triviality wf_state_add_d0g0v0_Shanghai_pre:
-  ∀c b r. wf_state (initial_state c add_d0g0v0_Shanghai_pre b r add_d0g0v0_Shanghai_transaction)
+Triviality wf_state_add_d0g0v0_Cancun_pre:
+  ∀c b r. wf_state (initial_state c add_d0g0v0_Cancun_pre b r add_d0g0v0_Cancun_transaction)
 Proof
-  ‘wf_accounts (add_d0g0v0_Shanghai_pre :160 word -> account_state)’
-    by (EVAL_TAC >> rw[])
+  ‘wf_accounts add_d0g0v0_Cancun_pre’ by (EVAL_TAC >> rw[])
   \\ rw[]
 QED
 
-Theorem add_d0g0v0_Shanghai_pre_code:
-  (add_d0g0v0_Shanghai_pre add_d0g0v0_Shanghai_transaction.to).code =
+Theorem add_d0g0v0_Cancun_pre_code:
+  (add_d0g0v0_Cancun_pre add_d0g0v0_Cancun_transaction.to).code =
   hex_to_bytes "600060006000600060006004356110000162fffffff100"
 Proof
-  simp[add_d0g0v0_Shanghai_pre_def, add_d0g0v0_Shanghai_transaction_def]
+  simp[add_d0g0v0_Cancun_pre_def, add_d0g0v0_Cancun_transaction_def,
+       update_account_def]
 QED
 
 fun cv_eval_match_tac pat =
@@ -184,19 +244,17 @@ fun eval_match_tac pat =
 Theorem lt_0_w2n_zero_bytes:
   (0 :num) >= w2n (word_of_bytes F (0w :256 word) [(0w :word8)])
 Proof
-  rw[byteTheory.word_of_bytes_def, byteTheory.set_byte_def]
-  \\ rw[wordsTheory.w2n_def]
-  \\ rw[byteTheory.set_byte_def]
+  cv_eval_match_tac ``word_of_bytes _ _ _``
   \\ EVAL_TAC
 QED
 
 Theorem memory_expansion_cost_d0g0v0:
   memory_expansion_cost [] (PAD_RIGHT 0w (32 * word_size 0) []) + 2630 ≤ 80000000
 Proof
-EVAL_TAC
+  EVAL_TAC
 QED
 
-val _ = mk_word_size 256
+val () = mk_word_size 256;
 
 Theorem set_byte_0ws:
   set_byte (0w:word256) 0w 0w e = 0w
@@ -211,31 +269,48 @@ Theorem assert_simps:
 Proof
   rw[assert_def]
 QED
-open  wordsTheory byteTheory arithmeticTheory;
-open wordsLib;
 
+val () = cv_auto_trans add_d0g0v0_Cancun_pre_def;
+val () = add_d0g0v0_Cancun_post_def |>
+  ONCE_REWRITE_RULE[GSYM update_storage_def] |>
+  cv_auto_trans;
+val () = cv_auto_trans add_d0g0v0_Cancun_transaction_def;
+val () = cv_auto_trans add_d0g0v0_Cancun_block_def;
 
-
-Theorem set_byte_word128[compute]:
-  set_byte (a:128 word) b (w:128 word) be =
-    let w0  = w2w (w >>> 64): 64 word in
-    let w0' = if w2n a >= 64 then set_byte (w2w a - 64w) b w0 be else w0 in
-    let w1 = w2w w: 64 word in
-    let w1' = if w2n a < 64 then set_byte (w2w a) b w1 be else w1 in
-    (w2w w0':128 word) << 64 || (w2w w1': 128 word)
+(*
+Theorem add_d0g0v0_Cancun_correctness:
+  ∃r. run (initial_state 1
+    add_d0g0v0_Cancun_pre
+    add_d0g0v0_Cancun_block
+    (Memory <| offset := 0; size := 0 |>)
+    add_d0g0v0_Cancun_transaction)
+  = SOME (Finished r) ∧ r.accounts = add_d0g0v0_Cancun_post
 Proof
-  cheat
-QED
+  rw[run_def, Once OWHILE_THM, PULL_EXISTS]
+  \\ cv_eval_match_tac ``step _``
+  \\ cv_eval_match_tac ``(Memory _)``
+  \\ cv_eval_match_tac ``(initial_state _ _ _ _ _)``
+  initial_state_def
+  cv_in
+  ff"initial_state""cv"
+  step_def
 
-val _ = byteTheory.byte_index_def |> INST_TYPE [alpha |-> “:64”] |> cv_trans;
-val _ = cv_trans byteTheory.set_byte_64;
-val _ = cv_trans set_byte_word128;
+  \\ rw[step_def]
+  \\ rw[Once bind_def]
+  \\ eval_match_tac “get_current_context _”
+  \\ rw[]
+  \\ qmatch_goalsub_abbrev_tac ‘pair_CASE (_ _ ctx) body’
+  \\ cv_eval_match_tac ``parse_opcode _`` \\ rw[]
+  \\ rw[bind_def, ignore_bind_def, assert_def]
+  \\ cv_eval_match_tac ``step_inst _``
 
-Theorem add_d0g0v0_Shanghai_correctness:
-  ∀c b rd.
-    ∃r. run (initial_state c add_d0g0v0_Shanghai_pre b rd add_d0g0v0_Shanghai_transaction)
-    = SOME (Finished r) ∧ r.accounts = add_d0g0v0_Shanghai_post
-Proof
+  initial_state_def
+  type_of``c.outputTo``
+  TypeBase.fields_of``:memory_range`` |> map type_of
+  type_of``Memory``
+  initial_tx_params_def
+  \\ cv_eval_match_tac ``step _``
+
   rpt (
     rw[run_def, Once OWHILE_THM, step_def]
     (* context *)
@@ -368,6 +443,8 @@ Proof
   \\ cheat
 QED
 Globals.max_print_depth := ~1;
+*)
+
 (*
 Definition CrashingTransaction_transaction_def:
   CrashingTransaction_transaction =
